format-version: 1.2
date: 13:01:2025 15:15
default-namespace: fermentdb_ontology

[Term]
id: FDBO:1
name: bioprocess variable
alt_id:
def: "" [url:http]
subset:
synonym: ""
xref:
is_a: 

[Term]
id: FDBO:2
name: cultivation condition
alt_id:
def: "An initial experimental parameter and/or environmental setting established prior to or at the start of a bioprocess. This condition, which may be categorical or scalar variable, can include key environmental setpoints such as pH, temperature (Tº), initial volume, and optical density (OD) of the seed culture" [url:http]
subset:
synonym: "cultivation_cond"
xref:
is_a: FDBO:1 ! bioprocess variable

[Term]
id: FDBO:3
name: process variable
alt_id:
def: "A technical parameter measured during a bioprocess, either through real-time (online, inline) or delayed (offline, atline) measurements, depending on the bioreactor setup. These variables are typically time-series data and are crucial for controlling and adjusting the initial parameters from cultivation conditions." [url:http]
subset:
synonym: "process_var"
xref:
is_a: DFBO:1 ! bioprocess variable

[Term]
id: FDBO:4
name: compound
alt_id:
def: "An offline bioprocess data refers to measurements obtained using instruments external to the bioreactor, such as High-Performance Liquid Chromatography (HPLC). These data typically include compound groups categorized as substrates, products, by-products, and chemical elements." [url:http]
subset:
synonym: ""
xref:
is_a: FDBO:1 ! bioprocess variable

[Term]
id: FDBO:5
name: calculated variable
alt_id:
def: "A computed variable that represents both intermediate and final results derived from bioprocess data. It is determined using initial parameters from cultivation conditions and process variables, including both online and offline measurements." [url:http]
subset:
synonym: "calculated_var"
xref:
is_a: FDBO:1 ! bioprocess variable

[Term]
id: FDBO:6
name: temperature_setpoint
alt_id:
def: "The target temperature value to be maintained within the fermenter, expressed in degrees celsius (ºC)."
subset:
synonym: "Temperature SetPoint (C)"
xref:
is_a: cultivation condition

